formalize padic taylor newton lift

lean4/BEDC/Derived/PadicUp/Hensel.lean
@@ -3,7 +3,9 @@ import BEDC.Derived.PadicUp.FieldCore
 namespace BEDC.Derived.PadicUp
 
 open BEDC.FKernel.Hist
+open BEDC.FKernel.Cont
 open BEDC.FKernel.Unary
+open BEDC.Derived.NatUp
 open BEDC.Derived.PrimeUp
 open BEDC.Derived.IntUp
 
@@ -18,17 +20,22 @@ def zpEval {p : BHist} : ZpPoly p -> ZpInt p -> ZpInt p
   | [c], _x => c
   | c :: d :: cs, x => zpAdd p c (zpMul p x (zpEval (d :: cs) x))
 
-def zpDerivAux {p : BHist} (prime : NatPrime p) : Nat -> ZpPoly p -> ZpPoly p
-  | _i, [] => []
-  | i, _c :: cs =>
-      match cs with
-      | [] => []
-      | d :: ds => zpMul p (zpNatCoeff prime (i + 1)) d :: zpDerivAux prime (i + 1) (d :: ds)
+def zpPolyAdd {p : BHist} : ZpPoly p -> ZpPoly p -> ZpPoly p
+  | [], ys => ys
+  | xs, [] => xs
+  | x :: xs, y :: ys => zpAdd p x y :: zpPolyAdd xs ys
+
+def zpPolyX {p : BHist} : ZpPoly p -> ZpPoly p
+  | [] => []
+  | c :: cs => zpZero p c.prime :: c :: cs
 
 def zpDeriv {p : BHist} (f : ZpPoly p) : ZpPoly p :=
   match f with
   | [] => []
-  | c :: cs => zpDerivAux c.prime 0 (c :: cs)
+  | [_c] => []
+  | _c :: d :: cs =>
+      let tail := d :: cs
+      zpPolyAdd tail (zpPolyX (zpDeriv tail))
 
 def zpLinearPoly {p : BHist} (b m : ZpInt p) : ZpPoly p :=
   [b, m]
@@ -50,12 +57,632 @@ theorem ZpUnit_of_ZpEq {p : BHist} {x y : ZpInt p} :
   exact unit (hsame_trans (hsame_symm (same (BHist.e1 BHist.Empty)
     (unary_e1_closed unary_empty))) sameZero)
 
+theorem zpAdd_rotate_middle {p : BHist} (a b c : ZpInt p) :
+    ZpEq (zpAdd p (zpAdd p a b) c) (zpAdd p (zpAdd p a c) b) := by
+  exact ZpEq_trans
+    (zpAdd_assoc p a b c)
+    (ZpEq_trans
+      (zpAdd_congr (ZpEq_refl a) (zpAdd_comm p b c))
+      (ZpEq_symm (zpAdd_assoc p a c b)))
+
+theorem zpAdd_pair_swap {p : BHist} (a b c d : ZpInt p) :
+    ZpEq (zpAdd p (zpAdd p a b) (zpAdd p c d))
+      (zpAdd p (zpAdd p a c) (zpAdd p b d)) := by
+  exact ZpEq_trans
+    (ZpEq_symm (zpAdd_assoc p (zpAdd p a b) c d))
+    (ZpEq_trans
+      (zpAdd_congr (zpAdd_rotate_middle a b c) (ZpEq_refl d))
+      (zpAdd_assoc p (zpAdd p a c) b d))
+
+theorem zpAdd_pair_to_left_nested {p : BHist} (a b c d : ZpInt p) :
+    ZpEq (zpAdd p (zpAdd p a b) (zpAdd p c d))
+      (zpAdd p (zpAdd p a (zpAdd p b c)) d) := by
+  exact ZpEq_trans
+    (ZpEq_symm (zpAdd_assoc p (zpAdd p a b) c d))
+    (zpAdd_congr (zpAdd_assoc p a b c) (ZpEq_refl d))
+
+theorem zpAdd_left_nested_four {p : BHist} (a b c d : ZpInt p) :
+    ZpEq (zpAdd p a (zpAdd p (zpAdd p b c) d))
+      (zpAdd p (zpAdd p (zpAdd p a b) c) d) := by
+  exact ZpEq_trans
+    (ZpEq_symm (zpAdd_assoc p a (zpAdd p b c) d))
+    (zpAdd_congr (ZpEq_symm (zpAdd_assoc p a b c)) (ZpEq_refl d))
+
+theorem zpTaylor_linear_terms {p : BHist} (a delta H D : ZpInt p) :
+    ZpEq
+      (zpAdd p (zpMul p delta H) (zpMul p a (zpMul p D delta)))
+      (zpMul p (zpAdd p H (zpMul p a D)) delta) := by
+  exact ZpEq_trans
+    (zpAdd_congr (zpMul_comm p delta H)
+      (ZpEq_symm (zpMul_assoc p a D delta)))
+    (ZpEq_symm (zpMul_add_distrib_right p H (zpMul p a D) delta))
+
+theorem zpTaylor_quadratic_middle {p : BHist} (delta D : ZpInt p) :
+    ZpEq (zpMul p delta (zpMul p D delta))
+      (zpMul p (zpMul p delta delta) D) := by
+  exact ZpEq_trans
+    (zpMul_right_congr (zpMul_comm p D delta))
+    (ZpEq_symm (zpMul_assoc p delta delta D))
+
+theorem zpTaylor_square_factor_left {p : BHist} (A delta g : ZpInt p) :
+    ZpEq (zpMul p A (zpMul p (zpMul p delta delta) g))
+      (zpMul p (zpMul p delta delta) (zpMul p A g)) := by
+  exact ZpEq_trans
+    (zpMul_comm p A (zpMul p (zpMul p delta delta) g))
+    (ZpEq_trans
+      (zpMul_assoc p (zpMul p delta delta) g A)
+      (zpMul_right_congr (zpMul_comm p g A)))
+
+theorem zpTaylor_tail_ring {p : BHist} (a delta H D g : ZpInt p) :
+    ZpEq
+      (zpMul p (zpAdd p a delta)
+        (zpAdd p (zpAdd p H (zpMul p D delta))
+          (zpMul p (zpMul p delta delta) g)))
+      (zpAdd p
+        (zpAdd p (zpMul p a H)
+          (zpMul p (zpAdd p H (zpMul p a D)) delta))
+        (zpMul p (zpMul p delta delta)
+          (zpAdd p D (zpMul p (zpAdd p a delta) g)))) := by
+  let A := zpAdd p a delta
+  let P := zpMul p delta delta
+  let Ddelta := zpMul p D delta
+  let linear := zpMul p (zpAdd p H (zpMul p a D)) delta
+  let quad := zpMul p P D
+  let Ag := zpMul p A g
+  let Pg := zpMul p P g
+  have outer :
+      ZpEq
+        (zpMul p A (zpAdd p (zpAdd p H Ddelta) Pg))
+        (zpAdd p (zpMul p A (zpAdd p H Ddelta)) (zpMul p A Pg)) :=
+    zpMul_add_distrib p A (zpAdd p H Ddelta) Pg
+  have firstExpand :
+      ZpEq
+        (zpMul p A (zpAdd p H Ddelta))
+        (zpAdd p (zpMul p A H) (zpMul p A Ddelta)) :=
+    zpMul_add_distrib p A H Ddelta
+  have aHExpand :
+      ZpEq (zpMul p A H)
+        (zpAdd p (zpMul p a H) (zpMul p delta H)) := by
+    unfold A
+    exact zpMul_add_distrib_right p a delta H
+  have dExpand :
+      ZpEq (zpMul p A Ddelta)
+        (zpAdd p (zpMul p a Ddelta) (zpMul p delta Ddelta)) := by
+    unfold A
+    exact zpMul_add_distrib_right p a delta Ddelta
+  have firstToExpanded :
+      ZpEq
+        (zpMul p A (zpAdd p H Ddelta))
+        (zpAdd p
+          (zpAdd p (zpMul p a H) (zpMul p delta H))
+          (zpAdd p (zpMul p a Ddelta) (zpMul p delta Ddelta))) :=
+    ZpEq_trans firstExpand (zpAdd_congr aHExpand dExpand)
+  have expandedToCompact :
+      ZpEq
+        (zpAdd p
+          (zpAdd p (zpMul p a H) (zpMul p delta H))
+          (zpAdd p (zpMul p a Ddelta) (zpMul p delta Ddelta)))
+        (zpAdd p (zpAdd p (zpMul p a H) linear) quad) := by
+    exact ZpEq_trans
+      (zpAdd_pair_to_left_nested (zpMul p a H) (zpMul p delta H)
+        (zpMul p a Ddelta) (zpMul p delta Ddelta))
+      (zpAdd_congr
+        (zpAdd_congr (ZpEq_refl _)
+          (by
+            unfold linear Ddelta
+            exact zpTaylor_linear_terms a delta H D))
+        (by
+          unfold quad P Ddelta
+          exact zpTaylor_quadratic_middle delta D))
+  have firstCompact :
+      ZpEq (zpMul p A (zpAdd p H Ddelta))
+        (zpAdd p (zpAdd p (zpMul p a H) linear) quad) :=
+    ZpEq_trans firstToExpanded expandedToCompact
+  have squareFactor :
+      ZpEq (zpMul p A Pg) (zpMul p P Ag) := by
+    unfold Pg P Ag A
+    exact zpTaylor_square_factor_left (zpAdd p a delta) delta g
+  have combineQuadratic :
+      ZpEq
+        (zpAdd p (zpAdd p (zpAdd p (zpMul p a H) linear) quad)
+          (zpMul p P Ag))
+        (zpAdd p (zpAdd p (zpMul p a H) linear)
+          (zpMul p P (zpAdd p D Ag))) := by
+    exact ZpEq_trans
+      (zpAdd_assoc p (zpAdd p (zpMul p a H) linear) quad (zpMul p P Ag))
+      (zpAdd_congr (ZpEq_refl _)
+        (ZpEq_symm (zpMul_add_distrib p P D Ag)))
+  exact ZpEq_trans outer
+    (ZpEq_trans
+      (zpAdd_congr firstCompact squareFactor)
+      combineQuadratic)
+
+theorem zpEval_poly_add {p : BHist} (f g : ZpPoly p) (x : ZpInt p) :
+    ZpEq (zpEval (zpPolyAdd f g) x)
+      (zpAdd p (zpEval f x) (zpEval g x)) := by
+  induction f generalizing g with
+  | nil =>
+      cases g with
+      | nil =>
+          change ZpEq (zpZero p x.prime)
+            (zpAdd p (zpZero p x.prime) (zpZero p x.prime))
+          exact ZpEq_symm (zpZero_add_left p x.prime (zpZero p x.prime))
+      | cons y ys =>
+          change ZpEq (zpEval (y :: ys) x)
+            (zpAdd p (zpZero p x.prime) (zpEval (y :: ys) x))
+          exact ZpEq_symm (zpZero_add_left p x.prime (zpEval (y :: ys) x))
+  | cons c cs ih =>
+      cases g with
+      | nil =>
+          change ZpEq (zpEval (c :: cs) x)
+            (zpAdd p (zpEval (c :: cs) x) (zpZero p x.prime))
+          exact ZpEq_symm (zpZero_add_right p x.prime (zpEval (c :: cs) x))
+      | cons d ds =>
+          cases cs with
+          | nil =>
+              cases ds with
+              | nil =>
+                  change ZpEq (zpAdd p c d) (zpAdd p c d)
+                  exact ZpEq_refl _
+              | cons e es =>
+                  change ZpEq
+                    (zpAdd p (zpAdd p c d) (zpMul p x (zpEval (e :: es) x)))
+                    (zpAdd p c
+                      (zpAdd p d (zpMul p x (zpEval (e :: es) x))))
+                  exact zpAdd_assoc p c d (zpMul p x (zpEval (e :: es) x))
+          | cons e es =>
+              cases ds with
+              | nil =>
+                  change ZpEq
+                    (zpAdd p (zpAdd p c d) (zpMul p x (zpEval (e :: es) x)))
+                    (zpAdd p (zpAdd p c (zpMul p x (zpEval (e :: es) x))) d)
+                  exact zpAdd_rotate_middle c d (zpMul p x (zpEval (e :: es) x))
+              | cons h hs =>
+                  change ZpEq
+                    (zpAdd p (zpAdd p c d)
+                      (zpMul p x (zpEval (zpPolyAdd (e :: es) (h :: hs)) x)))
+                    (zpAdd p (zpAdd p c (zpMul p x (zpEval (e :: es) x)))
+                      (zpAdd p d (zpMul p x (zpEval (h :: hs) x))))
+                  have tail :
+                      ZpEq
+                        (zpMul p x (zpEval (zpPolyAdd (e :: es) (h :: hs)) x))
+                        (zpMul p x
+                          (zpAdd p (zpEval (e :: es) x) (zpEval (h :: hs) x))) :=
+                    zpMul_right_congr (ih (h :: hs))
+                  exact ZpEq_trans
+                    (zpAdd_congr (ZpEq_refl _) tail)
+                    (ZpEq_trans
+                      (zpAdd_congr (ZpEq_refl _)
+                        (zpMul_add_distrib p x (zpEval (e :: es) x)
+                          (zpEval (h :: hs) x)))
+                      (zpAdd_pair_swap c d
+                        (zpMul p x (zpEval (e :: es) x))
+                        (zpMul p x (zpEval (h :: hs) x))))
+
+theorem zpEval_poly_x {p : BHist} (f : ZpPoly p) (x : ZpInt p) :
+    ZpEq (zpEval (zpPolyX f) x) (zpMul p x (zpEval f x)) := by
+  cases f with
+  | nil =>
+      change ZpEq (zpZero p x.prime) (zpMul p x (zpZero p x.prime))
+      exact ZpEq_symm (zpMul_zero_right p x)
+  | cons c cs =>
+      change ZpEq (zpAdd p (zpZero p c.prime) (zpMul p x (zpEval (c :: cs) x)))
+        (zpMul p x (zpEval (c :: cs) x))
+      exact zpZero_add_left p c.prime (zpMul p x (zpEval (c :: cs) x))
+
+theorem zpEval_congr_arg {p : BHist} (f : ZpPoly p) {x y : ZpInt p} :
+    ZpEq x y -> ZpEq (zpEval f x) (zpEval f y) := by
+  intro same
+  induction f with
+  | nil =>
+      exact ZpEq_refl _
+  | cons c tail ih =>
+      cases tail with
+      | nil =>
+          exact ZpEq_refl c
+      | cons d ds =>
+          change ZpEq
+            (zpAdd p c (zpMul p x (zpEval (d :: ds) x)))
+            (zpAdd p c (zpMul p y (zpEval (d :: ds) y)))
+          exact zpAdd_congr (ZpEq_refl c)
+            (zpMul_congr same ih)
+
+theorem taylor_remainder {p : BHist} (f : ZpPoly p) (a delta : ZpInt p) :
+    ∃ g : ZpInt p,
+      ZpEq (zpEval f (zpAdd p a delta))
+        (zpAdd p
+          (zpAdd p (zpEval f a) (zpMul p (zpEval (zpDeriv f) a) delta))
+          (zpMul p (zpMul p delta delta) g)) := by
+  induction f with
+  | nil =>
+      exact ⟨zpZero p a.prime, by
+        change ZpEq (zpZero p (zpAdd p a delta).prime)
+          (zpAdd p
+            (zpAdd p (zpZero p a.prime)
+              (zpMul p (zpZero p a.prime) delta))
+            (zpMul p (zpMul p delta delta) (zpZero p a.prime)))
+        exact ZpEq_symm
+          (ZpEq_trans
+            (zpAdd_congr
+              (ZpEq_trans
+                (zpAdd_congr (ZpEq_refl _)
+                  (zpMul_zero_left p a.prime delta))
+                (zpZero_add_right p a.prime (zpZero p a.prime)))
+              (zpMul_zero_right p (zpMul p delta delta)))
+            (zpZero_add_right p a.prime (zpZero p a.prime)))⟩
+  | cons c tail ih =>
+      cases tail with
+      | nil =>
+          exact ⟨zpZero p c.prime, by
+            change ZpEq c
+              (zpAdd p (zpAdd p c (zpMul p (zpZero p a.prime) delta))
+                (zpMul p (zpMul p delta delta) (zpZero p c.prime)))
+            exact ZpEq_symm
+              (ZpEq_trans
+                (zpAdd_congr
+                  (ZpEq_trans
+                    (zpAdd_congr (ZpEq_refl c)
+                      (zpMul_zero_left p a.prime delta))
+                    (zpZero_add_right p a.prime c))
+                  (zpMul_zero_right p (zpMul p delta delta)))
+                (zpZero_add_right p c.prime c))⟩
+      | cons d ds =>
+          cases ih with
+          | intro g hg =>
+              let H := zpEval (d :: ds) a
+              let D := zpEval (zpDeriv (d :: ds)) a
+              let P := zpMul p delta delta
+              let nextG := zpAdd p D (zpMul p (zpAdd p a delta) g)
+              have tailAt :
+                  ZpEq (zpEval (d :: ds) (zpAdd p a delta))
+                    (zpAdd p (zpAdd p H (zpMul p D delta)) (zpMul p P g)) :=
+                hg
+              have derivAt :
+                  ZpEq (zpEval (zpDeriv (c :: d :: ds)) a)
+                    (zpAdd p H (zpMul p a D)) := by
+                change ZpEq (zpEval (zpPolyAdd (d :: ds)
+                    (zpPolyX (zpDeriv (d :: ds)))) a)
+                  (zpAdd p H (zpMul p a D))
+                exact ZpEq_trans
+                  (zpEval_poly_add (d :: ds) (zpPolyX (zpDeriv (d :: ds))) a)
+                  (zpAdd_congr (ZpEq_refl H) (zpEval_poly_x (zpDeriv (d :: ds)) a))
+              exact ⟨nextG, by
+                change ZpEq
+                  (zpAdd p c
+                    (zpMul p (zpAdd p a delta)
+                      (zpEval (d :: ds) (zpAdd p a delta))))
+                  (zpAdd p
+                    (zpAdd p
+                      (zpAdd p c (zpMul p a H))
+                      (zpMul p (zpEval (zpDeriv (c :: d :: ds)) a) delta))
+                    (zpMul p P nextG))
+                have replaceTail :
+                    ZpEq
+                      (zpAdd p c
+                        (zpMul p (zpAdd p a delta)
+                          (zpEval (d :: ds) (zpAdd p a delta))))
+                      (zpAdd p c
+                        (zpMul p (zpAdd p a delta)
+                          (zpAdd p (zpAdd p H (zpMul p D delta))
+                            (zpMul p P g)))) :=
+                  zpAdd_congr (ZpEq_refl c) (zpMul_right_congr tailAt)
+                have ringStep :
+                    ZpEq
+                      (zpAdd p c
+                        (zpMul p (zpAdd p a delta)
+                          (zpAdd p (zpAdd p H (zpMul p D delta))
+                            (zpMul p P g))))
+                      (zpAdd p c
+                        (zpAdd p
+                          (zpAdd p (zpMul p a H)
+                            (zpMul p (zpAdd p H (zpMul p a D)) delta))
+                          (zpMul p P nextG))) :=
+                  zpAdd_congr (ZpEq_refl c) (zpTaylor_tail_ring a delta H D g)
+                have pack :
+                    ZpEq
+                      (zpAdd p c
+                        (zpAdd p
+                          (zpAdd p (zpMul p a H)
+                            (zpMul p (zpAdd p H (zpMul p a D)) delta))
+                          (zpMul p P nextG)))
+                      (zpAdd p
+                        (zpAdd p
+                          (zpAdd p c (zpMul p a H))
+                          (zpMul p (zpAdd p H (zpMul p a D)) delta))
+                        (zpMul p P nextG)) := by
+                  exact zpAdd_left_nested_four c (zpMul p a H)
+                    (zpMul p (zpAdd p H (zpMul p a D)) delta)
+                    (zpMul p P nextG)
+                exact ZpEq_trans replaceTail
+                  (ZpEq_trans ringStep
+                    (ZpEq_trans pack
+                      (zpAdd_congr
+                        (zpAdd_congr (ZpEq_refl _)
+                          (zpMul_left_congr (ZpEq_symm derivAt)))
+                        (ZpEq_refl _))))⟩
+
+theorem zpSub_self_cancel_left {p : BHist} (x y : ZpInt p) :
+    ZpEq (zpAdd p x (zpSub p y x)) y :=
+  zpAdd_sub_cancel x y
+
+theorem newton_delta_eq_neg {p : BHist} (f : ZpPoly p) (a : ZpInt p)
+    (unit : ZpUnit (zpEval (zpDeriv f) a)) :
+    ZpEq (zpSub p (newtonStep f a unit) a)
+      (zpNeg p (zpMul p (zpEval f a)
+        (ZpUnitInv (zpEval (zpDeriv f) a) unit))) := by
+  unfold newtonStep
+  unfold zpSub
+  let q := zpMul p (zpEval f a) (ZpUnitInv (zpEval (zpDeriv f) a) unit)
+  have assoc :
+      ZpEq (zpAdd p (zpAdd p a (zpNeg p q)) (zpNeg p a))
+        (zpAdd p a (zpAdd p (zpNeg p q) (zpNeg p a))) :=
+    zpAdd_assoc p a (zpNeg p q) (zpNeg p a)
+  have commute :
+      ZpEq (zpAdd p (zpNeg p q) (zpNeg p a))
+        (zpAdd p (zpNeg p a) (zpNeg p q)) :=
+    zpAdd_comm p (zpNeg p q) (zpNeg p a)
+  have assocBack :
+      ZpEq (zpAdd p a (zpAdd p (zpNeg p a) (zpNeg p q)))
+        (zpAdd p (zpAdd p a (zpNeg p a)) (zpNeg p q)) :=
+    ZpEq_symm (zpAdd_assoc p a (zpNeg p a) (zpNeg p q))
+  exact ZpEq_trans assoc
+    (ZpEq_trans (zpAdd_congr (ZpEq_refl a) commute)
+      (ZpEq_trans assocBack
+        (ZpEq_trans
+          (zpAdd_congr (zpAdd_neg_right p a) (ZpEq_refl (zpNeg p q)))
+          (zpZero_add_left p a.prime (zpNeg p q)))))
+
+theorem newton_d_times_q {p : BHist} (f : ZpPoly p) (a : ZpInt p)
+    (unit : ZpUnit (zpEval (zpDeriv f) a)) :
+    let fa := zpEval f a
+    let d := zpEval (zpDeriv f) a
+    let dinv := ZpUnitInv d unit
+    ZpEq (zpMul p d (zpMul p fa dinv)) fa := by
+  let fa := zpEval f a
+  let d := zpEval (zpDeriv f) a
+  let dinv := ZpUnitInv d unit
+  have assocForward :
+      ZpEq (zpMul p d (zpMul p fa dinv))
+        (zpMul p (zpMul p d fa) dinv) :=
+    ZpEq_symm (zpMul_assoc p d fa dinv)
+  have commuteLeft :
+      ZpEq (zpMul p (zpMul p d fa) dinv)
+        (zpMul p (zpMul p fa d) dinv) :=
+    zpMul_left_congr (zpMul_comm p d fa)
+  have assocBack :
+      ZpEq (zpMul p (zpMul p fa d) dinv)
+        (zpMul p fa (zpMul p d dinv)) :=
+    zpMul_assoc p fa d dinv
+  exact ZpEq_trans assocForward
+    (ZpEq_trans commuteLeft
+      (ZpEq_trans assocBack
+        (ZpEq_trans (zpMul_right_congr (ZpUnitInv_mul d unit))
+          (zpOne_mul_right p fa.prime fa))))
+
+theorem newton_linear_cancel {p : BHist} (f : ZpPoly p) (a : ZpInt p)
+    (unit : ZpUnit (zpEval (zpDeriv f) a)) :
+    ZpEq
+      (zpAdd p (zpEval f a)
+        (zpMul p (zpEval (zpDeriv f) a)
+          (zpSub p (newtonStep f a unit) a)))
+      (zpZero p (zpEval f a).prime) := by
+  let fa := zpEval f a
+  let d := zpEval (zpDeriv f) a
+  let dinv := ZpUnitInv d unit
+  let q := zpMul p fa dinv
+  have delta :
+      ZpEq (zpSub p (newtonStep f a unit) a) (zpNeg p q) :=
+    newton_delta_eq_neg f a unit
+  have replace :
+      ZpEq (zpMul p d (zpSub p (newtonStep f a unit) a))
+        (zpMul p d (zpNeg p q)) :=
+    zpMul_right_congr delta
+  have negTerm :
+      ZpEq (zpMul p d (zpNeg p q)) (zpNeg p fa) := by
+    apply zpAdd_cancel_right (z := zpMul p d q)
+    have rightZero :
+        ZpEq (zpAdd p (zpNeg p fa) (zpMul p d q))
+          (zpZero p fa.prime) := by
+      exact ZpEq_trans
+        (zpAdd_congr (ZpEq_refl (zpNeg p fa))
+          (newton_d_times_q f a unit))
+        (zpAdd_neg_left p fa)
+    have leftZero :
+        ZpEq (zpAdd p (zpMul p d (zpNeg p q)) (zpMul p d q))
+          (zpZero p d.prime) := by
+      have combine :
+          ZpEq (zpAdd p (zpMul p d (zpNeg p q)) (zpMul p d q))
+            (zpMul p d (zpAdd p (zpNeg p q) q)) :=
+        ZpEq_symm (zpMul_add_distrib p d (zpNeg p q) q)
+      exact ZpEq_trans combine
+        (ZpEq_trans (zpMul_right_congr (zpAdd_neg_left p q))
+          (zpMul_zero_right p d))
+    exact ZpEq_trans leftZero
+      (ZpEq_symm (ZpEq_trans rightZero
+        (zpZero_prime_irrel fa.prime d.prime)))
+  exact ZpEq_trans
+    (zpAdd_congr (ZpEq_refl fa)
+      (ZpEq_trans replace negTerm))
+    (zpAdd_neg_right p fa)
+
+theorem newton_step_as_add_delta {p : BHist} (f : ZpPoly p) (a : ZpInt p)
+    (unit : ZpUnit (zpEval (zpDeriv f) a)) :
+    ZpEq (newtonStep f a unit)
+      (zpAdd p a (zpSub p (newtonStep f a unit) a)) := by
+  exact ZpEq_symm (zpAdd_sub_cancel a (newtonStep f a unit))
+
+theorem newton_step_residual_square {p : BHist} (f : ZpPoly p) (a : ZpInt p)
+    (unit : ZpUnit (zpEval (zpDeriv f) a)) :
+    ∃ g : ZpInt p,
+      ZpEq (zpEval f (newtonStep f a unit))
+        (zpMul p
+          (zpMul p (zpSub p (newtonStep f a unit) a)
+            (zpSub p (newtonStep f a unit) a))
+          g) := by
+  let delta := zpSub p (newtonStep f a unit) a
+  cases taylor_remainder f a delta with
+  | intro g tg =>
+      have stepReplace :
+          ZpEq (zpEval f (newtonStep f a unit))
+            (zpEval f (zpAdd p a delta)) := by
+        exact zpEval_congr_arg f (newton_step_as_add_delta f a unit)
+      have collapse :
+          ZpEq
+            (zpAdd p
+              (zpAdd p (zpEval f a)
+                (zpMul p (zpEval (zpDeriv f) a) delta))
+              (zpMul p (zpMul p delta delta) g))
+            (zpMul p (zpMul p delta delta) g) := by
+        exact ZpEq_trans
+          (zpAdd_congr (newton_linear_cancel f a unit) (ZpEq_refl _))
+          (zpZero_add_left p (zpEval f a).prime (zpMul p (zpMul p delta delta) g))
+      exact ⟨g, ZpEq_trans stepReplace (ZpEq_trans tg collapse)⟩
+
+theorem NatMul_unit_left_closed_local {q : BHist} :
+    UnaryHistory q -> NatMul NatOne q q := by
+  intro qUnary
+  induction q with
+  | Empty =>
+      exact NatMul.zero (unary_e1_closed unary_empty)
+  | e0 q =>
+      cases qUnary
+  | e1 q ih =>
+      exact NatMul.succ (ih qUnary) (cont_intro rfl)
+
+theorem PDvdNat_zero_exponent {p n : BHist}
+    (prime : NatPrime p) (nUnary : UnaryHistory n) :
+    PDvdNat p (zpuNatToUnary 0) n := by
+  change PDvdNat p BHist.Empty n
+  exact ⟨NatOne, PPow.zero prime.left,
+    ⟨n, nUnary, NatMul_unit_left_closed_local nUnary⟩⟩
+
+theorem zpLevel_zero_to_PDvd_same {p : BHist} (a : ZpInt p)
+    (k : Nat)
+    (zeroK : (zpLevel a (zpuNatToUnary k) (zpuNatToUnary_unary k)).val =
+      BHist.Empty) :
+    PDvdNat p (zpuNatToUnary k)
+      (a.trunc (zpuNatToUnary k) (zpuNatToUnary_unary k)).val := by
+  have raw := zpLevel_zero_ext_PDvdNat a
+    (zpuNatToUnary_unary k) (zpuNatToUnary_unary 0) zeroK
+  change PDvdNat p (zpuNatToUnary k)
+    (a.trunc (BEDC.FKernel.Cont.append (zpuNatToUnary k) (zpuNatToUnary 0))
+      (unary_append_closed (zpuNatToUnary_unary k) (zpuNatToUnary_unary 0))).val at raw
+  have sameLevel :
+      hsame (BEDC.FKernel.Cont.append (zpuNatToUnary k) (zpuNatToUnary 0))
+        (zpuNatToUnary k) := by
+    exact append_empty_right (zpuNatToUnary k)
+  exact PDvdNat_hsame_exponent_result raw (hsame_refl _)
+    (zpTrunc_level_hsame a
+      (unary_append_closed (zpuNatToUnary_unary k) (zpuNatToUnary_unary 0))
+      (zpuNatToUnary_unary k) sameLevel)
+
+theorem zpMul_level_empty_of_left_level {p : BHist} (x y : ZpInt p)
+    (k : Nat)
+    (zeroX : (zpLevel x (zpuNatToUnary k) (zpuNatToUnary_unary k)).val =
+      BHist.Empty) :
+    (zpLevel (zpMul p x y) (zpuNatToUnary k) (zpuNatToUnary_unary k)).val =
+      BHist.Empty := by
+  have left : PDvdNat p (zpuNatToUnary k)
+      ((x.trunc (zpuNatToUnary k) (zpuNatToUnary_unary k)).val) :=
+    zpLevel_zero_to_PDvd_same x k zeroX
+  have right : PDvdNat p (zpuNatToUnary 0)
+      ((y.trunc (zpuNatToUnary k) (zpuNatToUnary_unary k)).val) :=
+    PDvdNat_zero_exponent y.prime
+      (BoundedNat_unary (pPowCanon_unary p (zpuNatToUnary k))
+        (y.trunc (zpuNatToUnary k) (zpuNatToUnary_unary k)))
+  have add : NatAdd (zpuNatToUnary k) (zpuNatToUnary 0) (zpuNatToUnary k) :=
+    ⟨zpuNatToUnary_unary k, zpuNatToUnary_unary 0,
+      cont_intro (append_empty_right (zpuNatToUnary k))⟩
+  exact zpMul_level_empty_of_PDvdNat_product x y (zpuNatToUnary_unary k)
+    add left right
+
+theorem ZpEq_level_empty_transport_local {p N : BHist} {x y : ZpInt p}
+    (NUnary : UnaryHistory N) :
+    ZpEq x y ->
+      (zpLevel y N NUnary).val = BHist.Empty ->
+        (zpLevel x N NUnary).val = BHist.Empty := by
+  intro same yZero
+  exact hsame_trans (same N NUnary) yZero
+
+theorem newton_delta_level_zero {p : BHist} (f : ZpPoly p) (a : ZpInt p)
+    (unit : ZpUnit (zpEval (zpDeriv f) a)) (k : Nat)
+    (faZero : (zpLevel (zpEval f a) (zpuNatToUnary k)
+      (zpuNatToUnary_unary k)).val = BHist.Empty) :
+    (zpLevel (zpSub p (newtonStep f a unit) a) (zpuNatToUnary k)
+      (zpuNatToUnary_unary k)).val = BHist.Empty := by
+  let fa := zpEval f a
+  let d := zpEval (zpDeriv f) a
+  let dinv := ZpUnitInv d unit
+  have qZero :
+      (zpLevel (zpMul p fa dinv) (zpuNatToUnary k)
+        (zpuNatToUnary_unary k)).val = BHist.Empty :=
+    zpMul_level_empty_of_left_level fa dinv k faZero
+  have deltaEq :
+      ZpEq (zpSub p (newtonStep f a unit) a)
+        (zpNeg p (zpMul p fa dinv)) :=
+    newton_delta_eq_neg f a unit
+  have negZero :
+      (zpLevel (zpNeg p (zpMul p fa dinv)) (zpuNatToUnary k)
+        (zpuNatToUnary_unary k)).val = BHist.Empty := by
+    have addDrop :
+        hsame ((zpAdd p (zpNeg p (zpMul p fa dinv)) (zpMul p fa dinv)).trunc
+          (zpuNatToUnary k) (zpuNatToUnary_unary k)).val
+          ((zpNeg p (zpMul p fa dinv)).trunc
+            (zpuNatToUnary k) (zpuNatToUnary_unary k)).val :=
+      zpAdd_level_zero_right (zpNeg p (zpMul p fa dinv)) (zpMul p fa dinv)
+        (zpuNatToUnary_unary k) qZero
+    have addZero :
+        hsame ((zpAdd p (zpNeg p (zpMul p fa dinv)) (zpMul p fa dinv)).trunc
+          (zpuNatToUnary k) (zpuNatToUnary_unary k)).val
+          ((zpZero p (zpMul p fa dinv).prime).trunc
+            (zpuNatToUnary k) (zpuNatToUnary_unary k)).val :=
+      zpAdd_neg_left p (zpMul p fa dinv) (zpuNatToUnary k) (zpuNatToUnary_unary k)
+    exact hsame_trans (hsame_symm addDrop) addZero
+  exact ZpEq_level_empty_transport_local (zpuNatToUnary_unary k) deltaEq negZero
+
+theorem newton_step_lifts {p : BHist} (f : ZpPoly p) (a : ZpInt p)
+    (unit : ZpUnit (zpEval (zpDeriv f) a)) (k : Nat)
+    (faZero : (zpLevel (zpEval f a) (zpuNatToUnary k)
+      (zpuNatToUnary_unary k)).val = BHist.Empty) :
+    (zpLevel (zpEval f (newtonStep f a unit)) (zpuNatToUnary (k + k))
+      (zpuNatToUnary_unary (k + k))).val = BHist.Empty := by
+  cases newton_step_residual_square f a unit with
+  | intro g residual =>
+      let delta := zpSub p (newtonStep f a unit) a
+      let N := zpuNatToUnary (k + k)
+      have NUnary : UnaryHistory N := zpuNatToUnary_unary (k + k)
+      have deltaZero :
+          (zpLevel delta (zpuNatToUnary k) (zpuNatToUnary_unary k)).val =
+            BHist.Empty :=
+        newton_delta_level_zero f a unit k faZero
+      have leftRaw : PDvdNat p (zpuNatToUnary k)
+          (delta.trunc N NUnary).val := by
+        have appendSame :
+            hsame (BEDC.FKernel.Cont.append (zpuNatToUnary k) (zpuNatToUnary k)) N :=
+          zpuNatToUnary_add_hsame k k
+        have raw := zpLevel_zero_ext_PDvdNat delta
+          (zpuNatToUnary_unary k) (zpuNatToUnary_unary k) deltaZero
+        exact PDvdNat_hsame_exponent_result raw (hsame_refl _)
+          (zpTrunc_level_hsame delta
+            (unary_append_closed (zpuNatToUnary_unary k) (zpuNatToUnary_unary k))
+            NUnary appendSame)
+      have squareZero :
+          (zpLevel (zpMul p delta delta) N NUnary).val = BHist.Empty := by
+        exact zpMul_level_empty_of_PDvdNat_product delta delta NUnary
+          (zpuNatToUnary_natAdd k k) leftRaw leftRaw
+      have squareTimesZero :
+          (zpLevel (zpMul p (zpMul p delta delta) g) N NUnary).val =
+            BHist.Empty :=
+        zpMul_level_empty_of_left_level (zpMul p delta delta) g (k + k)
+          squareZero
+      exact ZpEq_level_empty_transport_local NUnary residual squareTimesZero
+
 theorem zpEval_linear {p : BHist} (b m x : ZpInt p) :
     ZpEq (zpEval (zpLinearPoly b m) x) (zpAdd p b (zpMul p x m)) := by
   exact ZpEq_refl _
 
 theorem zpDeriv_linear {p : BHist} (b m : ZpInt p) :
-    zpDeriv (zpLinearPoly b m) = [zpMul p (zpNatCoeff b.prime 1) m] := by
+    zpDeriv (zpLinearPoly b m) = [m] := by
   rfl
 
 theorem zpNatCoeff_one_mul {p : BHist} (prime : NatPrime p) (x : ZpInt p) :
@@ -65,8 +692,7 @@ theorem zpNatCoeff_one_mul {p : BHist} (prime : NatPrime p) (x : ZpInt p) :
 
 theorem zpEval_deriv_linear {p : BHist} (b m x : ZpInt p) :
     ZpEq (zpEval (zpDeriv (zpLinearPoly b m)) x) m := by
-  change ZpEq (zpMul p (zpNatCoeff b.prime 1) m) m
-  exact zpNatCoeff_one_mul b.prime m
+  exact ZpEq_refl m
 
 def linearHenselUnit {p : BHist} (b m a0 : ZpInt p) (unit : ZpUnit m) :
     ZpUnit (zpEval (zpDeriv (zpLinearPoly b m)) a0) :=
